coq-SystemRF-1.1/Denotations/BasicPropsDenotes.v
@@ -1,15 +1,21 @@
 Require Import SystemRF.BasicDefinitions.
 Require Import SystemRF.Names.
 Require Import SystemRF.Strengthenings.
+Require Import SystemRF.LocalClosure.
 Require Import SystemRF.Semantics.
 Require Import SystemRF.SystemFTyping.
 Require Import SystemRF.WellFormedness.
 Require Import SystemRF.BasicPropsSubstitution.
 Require Import SystemRF.BasicPropsEnvironments.
 Require Import SystemRF.BasicPropsWellFormedness.
+Require Import SystemRF.Typing.
+Require Import SystemRF.LemmasTransitive.
 Require Import Denotations.ClosingSubstitutions.
 Require Import Denotations.Denotations.
+Require Import Denotations.PrimitivesSemantics.
 Require Import Denotations.BasicPropsCSubst.
+
+Require Import Arith.
 
 Lemma lem_denotesenv_loc_closed : forall (g:env) (th:csub), 
     DenotesEnv g th -> loc_closed th.
@@ -33,3 +39,255 @@ Lemma lem_denotesenv_substitutable : forall (g:env) (th:csub),
     DenotesEnv g th -> substitutable th.
 Proof. intros; induction H; simpl; try split; trivial.
   apply lem_den_isvalue with (ctsubst th t); apply H1. Qed.
+
+
+(* Unfortunately, the self operator and tsubFTV do not quite 
+   commute with each other, but are entirely semantically 
+   equivalent. The next lemma shows that the denotation is
+   unaffected (used to prove Denotational Soundness)
+*)
+
+Lemma lem_erase_tsubFTV_self :
+  forall (a:vname) (t_a t:type) (v:expr) (k :kind),
+    noExists t_a -> erase (self (tsubFTV a t_a t) v k) 
+                      = erase (tsubFTV a t_a (self t v k)).
+Proof. intros a t_a; induction t; intros v k' H;
+  destruct k'; repeat rewrite lem_self_star; trivial;
+  try destruct b eqn:B; simpl;
+  try destruct (a =? a0) eqn:A; simpl; try reflexivity.
+  - (* TRefn Base *) destruct t_a; simpl in H; simpl;
+    try contradiction; reflexivity.
+  - (* TExists Base *) apply IHt2; apply H.
+  Qed.
+
+Lemma lem_denotes_tsubFTV_self' : 
+  forall (n:nat) (a:vname) (t_a t:type) (v v':expr) (k:kind),
+    depth t <= n -> noExists t_a -> isLCT t_a -> freeTV t_a = empty
+        -> subFTV a t_a v = v -> isLC v
+        -> Denotes (self (tsubFTV a t_a t)  v  k) v'
+        -> Denotes (tsubFTV a t_a (self t v k)) v'.
+Proof. induction n.
+  - (* n = 0 => TRefn *) intros; revert H5;
+    assert (depth t = 0) by auto with *;
+    destruct t; simpl in H5; try discriminate;
+    destruct k; try rewrite lem_self_star; trivial. 
+    destruct b; simpl; rewrite H3;
+    unfold eqlPred; trivial. (* FTV a0 remains*)
+    destruct (a =? a0) eqn:A; simpl; 
+    unfold eqlPred; trivial.
+    (* a = a0*) destruct t_a; simpl in A; try contradiction;
+    simpl; trivial; unfold eqlPred.
+    repeat rewrite Denotes_equation_1; intuition.
+    apply PECons; fold subBV_at; fold psubBV_at;
+    inversion H9; try apply H12. 
+    destruct (0 =? 0) eqn:Z; simpl in Z; try discriminate;
+    destruct b eqn:B; unfold isLCT in H1; simpl in H2;
+    try destruct i; try destruct H1; try inversion H1;
+    try apply (empty_no_elem (names_add a1 (ftvP ps0))) with a1 in H2;
+    try apply not_elem_names_add_elim in H2; try destruct H2; intuition.
+    * (* TBool *) 
+      apply AddStep with (App (App (Prim Eqv) (subBV_at 0 v' v)) v').
+      apply EApp1; apply EApp1; apply lem_step_eql_tbool.
+      apply lem_decompose_evals with 
+        (App (App (AppT (Prim Eql) (TRefn TBool PEmpty)) (subBV_at 0 v' v)) v');
+      trivial; apply lem_step_evals;
+      apply EApp1; apply EApp1; apply lem_step_eql_tbool.
+    * (* TInt *) 
+      apply AddStep with (App (App (Prim Eq) (subBV_at 0 v' v)) v').
+      apply EApp1; apply EApp1; apply lem_step_eql_tint.
+      apply lem_decompose_evals with 
+        (App (App (AppT (Prim Eql) (TRefn TInt PEmpty)) (subBV_at 0 v' v)) v');
+      trivial; apply lem_step_evals;
+      apply EApp1; apply EApp1; apply lem_step_eql_tint.
+  - (* n > 0 *) intros; destruct t.
+    * (* TRefn *) apply IHn; revert H5; simpl; auto with *.
+    * (* TFunc *) destruct k; simpl; simpl in H5; apply H5.
+    * (* TExists *) revert H5; destruct k; simpl; trivial.
+      (* Base *) repeat rewrite Denotes_equation_3;
+      simpl; rewrite lem_erase_tsubFTV_self; intuition;
+      destruct H8 as [v_x H8]; exists v_x; intuition.
+      rewrite lem_tsubBV_self in H10; trivial.
+      apply lem_den_hasftype in H8 as H9.
+      apply lem_fv_subset_bindsF in H9 as H9;
+      destruct H9; unfold Subset in H11; simpl in H11;
+      assert (subFTV a t_a v_x = v_x)
+        by (apply lem_subFTV_notin; unfold not; apply H11). 
+      trivial || rewrite <- H12; rewrite <- H12 in H10.
+      rewrite <- lem_commute_tsubFTV_tsubBV in H10;
+      try rewrite <- lem_commute_tsubFTV_tsubBV;
+      try assumption; rewrite lem_tsubBV_self;
+      try apply IHn; simpl in H; apply Nat.succ_le_mono in H;
+      try rewrite depth_tsubBV;
+      try apply Nat.le_trans with (max (depth t1) (depth t2));
+      try apply Nat.le_max_r;
+      unfold isLC; simpl; trivial.
+    * (* TPoly *) destruct k; simpl; simpl in H5; apply H5.
+  Qed.
+  
+Lemma lem_denotes_tsubFTV_self : 
+  forall (a:vname) (t_a t:type) (v v':expr) (k:kind),
+    noExists t_a -> isLCT t_a -> freeTV t_a = empty
+        -> subFTV a t_a v = v -> isLC v
+        -> Denotes (self (tsubFTV a t_a t) v k) v'
+        -> Denotes (tsubFTV a t_a (self t v k)) v'.
+Proof. intros a t_a t v v' k.
+  apply lem_denotes_tsubFTV_self' with (depth t); trivial. Qed.
+
+Lemma lem_denotes_ctsubst_self : 
+  forall (th:csub) (t:type) (v v':expr) (k:kind),
+    closed th -> loc_closed th -> substitutable th
+        -> Denotes (self (ctsubst th t) (csubst th v) k) v'
+        -> Denotes (ctsubst th (self t v k)) v'.
+Proof. induction th; intros t v v' k H1 H2 H3; simpl; trivial.
+  - (* CCons *) rewrite lem_tsubFV_self; apply IHth; auto with *.
+  - (* CConsT *) intros; simpl in H1; simpl in H2; simpl in H3;
+    destruct H1; destruct H1; destruct H2; destruct H3;
+    pose proof (matchesExFTV_dec a t) as Hm; destruct Hm.
+    * (* Yes *) destruct t; try destruct b; simpl in H7;
+      try contradiction; try subst a0.
+
+    * (* No *)
+
+
+Lemma lem_tsubFTV_matches : forall (a:vname) (t_a t:type),
+    freeTV t_a = empty -> noExists t_a
+        -> matchesExFTV a t -> ~ isExFTV (tsubFTV a t_a t).
+Lemma lem_tsubFTV_self_noFTV : forall (a:vname) (t_a t:type) (v:expr) (k:kind),
+    ~ matchesExFTV a t 
+      -> tsubFTV a t_a (self t v k) = self (tsubFTV a t_a t) (subFTV a t_a v) k.
+Lemma lem_ctsubst_self_noFTV : forall (th:csub) (t:type) (v:expr) (k:kind),
+    ~ isExFTV t -> ctsubst th (self t v k) = self (ctsubst th t) (csubst th v) k.
+
+Lemma lem_denotes_ctsubst_tsubFTV_self : 
+  forall (th:csub) (a:vname) (t_a t:type) (v v':expr) (k:kind),
+    closed th -> loc_closed th -> substitutable th
+        -> noExists t_a -> isLCT t_a -> free t_a = empty -> freeTV t_a = empty
+        -> ftv v = empty -> isLC v
+        -> Denotes (ctsubst th (self (tsubFTV a t_a t) v k)) v'
+        -> Denotes (ctsubst th (tsubFTV a t_a (self t v k))) v'.
+Proof. induction th; intros; revert H8; simpl.
+  - (* CEmpty *) apply lem_denotes_tsubFTV_self;
+    try apply lem_subFTV_notin; try apply empty_no_elem; trivial.
+  - (* CCons *) rewrite lem_commute_tsubFV_tsubFTV;
+    try repeat rewrite lem_tsubFV_self;
+    try rewrite lem_commute_tsubFV_tsubFTV; try apply IHth;
+    simpl in H; simpl in H0; simpl in H1; 
+    try apply lem_islc_at_subFV;
+    destruct H; destruct H0; destruct H1; destruct H8;
+    try apply empty_no_elem; trivial;
+    assert (Subset (ftv (subFV x v_x v)) (union empty empty))
+        by (rewrite <- H6 at 1; rewrite <- H8; apply ftv_subFV_elim);
+    apply no_elem_empty; intros; 
+    apply not_elem_subset with (union empty empty); auto.
+  - (* CConsT *)
+
+
+
+    
+  apply lem_denotes_tsubFTV_self' with (depth t); trivial. Qed.  
+
+
+
+x v' k'; destruct k'; simpl;
+    try rewrite lem_ctsubst_func; try rewrite lem_ctsubst_exis;
+    try rewrite lem_ctsubst_poly; simpl; trivial.
+    - (* TRefn Base *)
+
+    (* maybe try with subFTV first in the Basic Props Denotes file?*)  
+
+
+
+
+
+
+
+
+
+
+
+
+
+
+
+
+
+
+
+
+
+
+
+
+
+
+
+
+
+
+
+Lemma lem_denotes_ctsubst_self' : 
+  forall (n:nat) (th:csub) (t:type) (v v':expr) (k:kind),
+    depth t <= n -> closed th -> loc_closed th -> substitutable th
+        -> isLC v
+        -> Denotes (self (ctsubst th t) (csubst th v) k) v'
+        -> Denotes (ctsubst th (self t v k)) v'.
+Proof. induction n.
+  - (* n = 0 => TRefn *) induction th;
+    intros; revert H4;
+    assert (depth t = 0) by auto with *;
+    destruct t; simpl in H4; try discriminate;
+    destruct k; try rewrite lem_self_star; trivial.
+    
+    simpl. 
+    destruct b; simpl. ; rewrite H3;
+    unfold eqlPred; trivial. (* FTV a0 remains*)
+    destruct (a =? a0) eqn:A; simpl; 
+    unfold eqlPred; trivial.
+    (* a = a0*) destruct t_a; simpl in A; try contradiction;
+    simpl; trivial; unfold eqlPred.
+    repeat rewrite Denotes_equation_1; intuition.
+    apply PECons; fold subBV_at; fold psubBV_at;
+    inversion H9; try apply H12. 
+    destruct (0 =? 0) eqn:Z; simpl in Z; try discriminate;
+    destruct b eqn:B; unfold isLCT in H1; simpl in H2;
+    try destruct i; try destruct H1; try inversion H1;
+    try apply (empty_no_elem (names_add a1 (ftvP ps0))) with a1 in H2;
+    try apply not_elem_names_add_elim in H2; try destruct H2; intuition.
+    * (* TBool *) 
+      apply AddStep with (App (App (Prim Eqv) (subBV_at 0 v' v)) v').
+      apply EApp1; apply EApp1; apply lem_step_eql_tbool.
+      apply lem_decompose_evals with 
+        (App (App (AppT (Prim Eql) (TRefn TBool PEmpty)) (subBV_at 0 v' v)) v');
+      trivial; apply lem_step_evals;
+      apply EApp1; apply EApp1; apply lem_step_eql_tbool.
+    * (* TInt *) 
+      apply AddStep with (App (App (Prim Eq) (subBV_at 0 v' v)) v').
+      apply EApp1; apply EApp1; apply lem_step_eql_tint.
+      apply lem_decompose_evals with 
+        (App (App (AppT (Prim Eql) (TRefn TInt PEmpty)) (subBV_at 0 v' v)) v');
+      trivial; apply lem_step_evals;
+      apply EApp1; apply EApp1; apply lem_step_eql_tint.
+  - (* n > 0 *) intros; destruct t.
+    * (* TRefn *) apply IHn; revert H5; simpl; auto with *.
+    * (* TFunc *) destruct k; simpl; simpl in H5; apply H5.
+    * (* TExists *) revert H5; destruct k; simpl; trivial.
+      (* Base *) repeat rewrite Denotes_equation_3;
+      simpl; rewrite lem_erase_tsubFTV_self; intuition;
+      destruct H8 as [v_x H8]; exists v_x; intuition.
+      rewrite lem_tsubBV_self in H10; trivial.
+      apply lem_den_hasftype in H8 as H9.
+      apply lem_fv_subset_bindsF in H9 as H9;
+      destruct H9; unfold Subset in H11; simpl in H11;
+      assert (subFTV a t_a v_x = v_x)
+        by (apply lem_subFTV_notin; unfold not; apply H11). 
+      trivial || rewrite <- H12; rewrite <- H12 in H10.
+      rewrite <- lem_commute_tsubFTV_tsubBV in H10;
+      try rewrite <- lem_commute_tsubFTV_tsubBV;
+      try assumption; rewrite lem_tsubBV_self;
+      try apply IHn; simpl in H; apply Nat.succ_le_mono in H;
+      try rewrite depth_tsubBV;
+      try apply Nat.le_trans with (max (depth t1) (depth t2));
+      try apply Nat.le_max_r;
+      unfold isLC; simpl; trivial.
+    * (* TPoly *) destruct k; simpl; simpl in H5; apply H5.
+  Qed.    
