coq-SystemRF-1.1/Denotations/SelfifyDenotations.v
@@ -1,139 +1,97 @@
 Require Import SystemRF.BasicDefinitions.
 Require Import SystemRF.Names.
+Require Import SystemRF.Semantics.
 Require Import SystemRF.SystemFTyping.
+Require Import SystemRF.PrimitivesFTyping.
 Require Import SystemRF.WellFormedness.
 Require Import SystemRF.Typing.
-(*Require Import SystemRF.BasicPropsSubstitution.
-Require Import SystemRF.BasicPropsEnvironments.*)
+Require Import SystemRF.BasicPropsSubstitution.
+Require Import SystemRF.BasicPropsEnvironments.
+Require Import SystemRF.BasicPropsWellFormedness.
+Require Import SystemRF.SubstitutionLemmaWF.
+Require Import SystemRF.LemmasTransitive.
 Require Import Denotations.ClosingSubstitutions.
 Require Import Denotations.Denotations.
 Require Import Denotations.BasicPropsCSubst.
 Require Import Denotations.PrimitivesSemantics.
+Require Import Denotations.PrimitivesDenotations.
 
-(*
-{-@ lem_denotations_selfify_trefn :: b:Basic -> z:RVname -> p:Pred 
-        -> ProofOf(WFType Empty (TRefn b z p) Base) -> { e:Term | Set_emp (freeBV e) } 
-        -> ProofOf(HasFType FEmpty e (FTBasic b)) -> v:Value -> ProofOf(EvalsTo e v) 
-        -> ProofOf(Denotes (TRefn b z p) v) -> ProofOf(Denotes (self (TRefn b z p) e Base) v) @-}
-lem_denotations_selfify_trefn :: Basic -> RVname -> Expr -> WFType -> Expr -> HasFType -> Expr
-                                -> EvalsTo -> Denotes -> Denotes
-lem_denotations_selfify_trefn b z p p_emp_t e p_e_t v ev_e_v den_t_v 
-  = DRefn b z (strengthen  (App (App (AppT (Prim Eql) (TRefn b z p)) (BV 0)) e)  p) --(selfify p b z e) 
-          v p_v_b (ev_selfpv_tt
-          ? lem_subBV_strengthen 0 v (App (App (AppT (Prim Eql) (TRefn b z p)) (BV 0)) e) p
-          ? lem_subBV_notin 0 v e
-          ? lem_tsubBV_notin 0 v (TRefn b z p) )
-      where
-        (DRefn _b _z _p _v p_v_b ev_pv_tt) = den_t_v
-        y_           = fresh_var Empty
-        y            = y_ ? lem_free_bound_in_env Empty (TRefn b z p) Base p_emp_t y_
-                          ? lem_fv_bound_in_fenv FEmpty e (FTBasic b) p_e_t y_
-        {-@ ev_rhs_tt :: ProofOf(EvalsTo (App (App (AppT (Prim Eql) (TRefn b z p)) v) e) 
-                                         (Bc True)) @-}
-        ev_rhs_tt    = lem_equals_evals b z p e v ev_e_v p_v_b 
-        p_eqlte_b    = lem_eqlPred_ftyping Empty b z p p_emp_t WFFEmpty y e p_e_t 
-        p_emp_er_t   = lem_erase_wftype Empty (TRefn b z p)  Base p_emp_t
-        p_y_wf       = WFFBind FEmpty WFFEmpty y (FTBasic b) Base p_emp_er_t
-        {-@ p_eqltev_b :: ProofOf(HasFType FEmpty 
-                                           (App (App (AppT (Prim Eql) (TRefn b z p)) v) e) 
-                                           (FTBasic TBool)) @-}
-        p_eqltev_b   = lem_subst_ftyp FEmpty FEmpty y v (FTBasic b) p_v_b p_y_wf
-                                      (App (App (AppT (Prim Eql) (TRefn b z p)) (FV y)) e) 
-                                      (FTBasic TBool) p_eqlte_b 
-                           ? lem_subFV_notin y v e
-                           ? lem_subFV_notin y v p
-                           ? lem_empty_concatF FEmpty
-        {-@ ev_selfpv_tt :: ProofOf(EvalsTo 
-                          (strengthen  (App (App (AppT (Prim Eql) (TRefn b z p)) v) e)  (subBV 0 v p)) 
-                          (Bc True)) @-}
-        ev_selfpv_tt = lem_strengthen_evals_tt (App (App (AppT (Prim Eql) (TRefn b z p)) v) e) 
-                                               (subBV 0 v p) p_eqltev_b ev_rhs_tt ev_pv_tt
+Require Import Arith.
 
---- Lemma 7 in the paper version
-{-@ lem_denotations_selfify :: t:Type -> k:Kind -> ProofOf(WFType Empty t k)
-        -> { e:Term | Set_emp (freeBV e) } -> ProofOf(HasFType FEmpty e (erase t))
-        -> v:Value -> ProofOf(EvalsTo e v) -> ProofOf(Denotes t v)
-        -> ProofOf(Denotes (self t e k) v) @-}
-lem_denotations_selfify :: Type -> Kind -> WFType -> Expr -> HasFType -> Expr
-                                -> EvalsTo -> Denotes -> Denotes
-lem_denotations_selfify t@(TRefn b z p)    Base p_emp_t e p_e_t v ev_e_v den_t_v 
-  = lem_denotations_selfify_trefn b z (p ? lem_refn_is_pred t b z p) p_emp_t 
-                                  e p_e_t v ev_e_v den_t_v
-lem_denotations_selfify (TFunc z t_z t')   k    p_emp_t e p_e_t v ev_e_v den_t_v = den_t_v
-lem_denotations_selfify (TExists z t_z t') Base p_emp_t e p_e_t v ev_e_v den_t_v = case den_t_v of
-  (DExis _z _tz _t' _v p_v_ert' v_z den_tz_vz den_t'vz_v) 
-    -> DExis z t_z (self t' e Base) v p_v_ert' v_z den_tz_vz den_selft'vz_v
-         where 
-           p_vz_er_tz     = get_ftyp_from_den t_z v_z den_tz_vz
-           (WFExis _ _ _ k_z p_g_tz _ k_t' y p_y_t')
-                          = lem_wfexis_for_wf_texists Empty  z t_z t' Base p_emp_t 
-           p_y_wf         = WFEBind Empty WFEEmpty y t_z k_z p_g_tz
-           p_emp_t'vz     = lem_subst_wf Empty Empty y v_z t_z p_vz_er_tz p_y_wf 
-                                         (unbindT z y t') k_t' p_y_t'
-                                         ? lem_empty_concatE Empty
-                                         ? lem_tsubFV_unbindT z y v_z t'
-           den_selft'vz_v = lem_denotations_selfify (tsubBV z v_z t') k_t' p_emp_t'vz 
-                                                    e (p_e_t ? lem_erase_tsubBV z v_z t')
-                                                    v ev_e_v den_t'vz_v
-                                                    ? lem_tsubBV_self z v_z t' e Base
-lem_denotations_selfify (TPoly a k_a t')   k    p_emp_t e p_e_t v ev_e_v den_t_v = den_t_v
-lem_denotations_selfify t                  Star p_emp_t e p_e_t v ev_e_v den_t_v = den_t_v
+Lemma lem_denotations_selfify' : forall (n:nat) (g:env) (t:type) (k:kind) (v:expr),
+    depth t <= n -> WFtype g t k -> g = Empty 
+        -> HasFtype FEmpty v (erase t) -> isValue v
+        -> Denotes t v -> Denotes (self t v k) v.
+Proof. induction n.
+  - (* n = 0 => TRefn *) intros; 
+    assert (depth t = 0) by auto with *.
+    destruct t; simpl in H5; try discriminate;
+    clear H H5; subst g;
+    destruct k; simpl; simpl in H2.
+    * (* k = Base *) rewrite Denotes_equation_1.
+      unfold psubBV; simpl; inversion H4; destruct H1;    
+      simpl in H1; repeat split; try apply PECons;
+      try assumption.
+      apply lem_ftyp_islc in H1 as Hv; rewrite lem_subBV_lc; 
+      try apply Hv.
+      assert (isClosedBasic b) as Hb
+        by (destruct b; inversion H0; simpl in H8; inversion H8; 
+            try simpl in H14; try contradiction; trivial).
+      destruct b eqn:B; simpl in Hb; try contradiction.
+      + (* Bool *) assert (isBool v)
+          by (apply lem_den_bools with (TRefn TBool ps); simpl; trivial);
+        destruct v eqn:V; try contradiction.
+        assert (true = Bool.eqb b0 b0) by (destruct b0; reflexivity);
+        rewrite H7; apply lemma_eql_bool_semantics; apply Refl.
+      + (* Int *) assert (isInt v)
+          by (apply lem_den_ints with (TRefn TInt ps); simpl; trivial);
+        destruct v eqn:V; try contradiction.
+        assert ((n =? n) = true) by (apply Nat.eqb_eq; reflexivity);
+        rewrite <- H7; apply lemma_eql_int_semantics; apply Refl.
+    * (* k = Star *) apply H4.
+  - (* n > 0 *) intros; subst g; destruct t.
+    * (* TRefn *) apply IHn with Empty; simpl in H2;
+      simpl; auto with *. 
+    * (* TFunc *) destruct k; simpl; apply H4.
+    * (* TExis *) destruct k.
+      + (* Base *) simpl; rewrite Denotes_equation_3; simpl; 
+        rewrite lem_erase_self; repeat split; try assumption.
+        rewrite Denotes_equation_3 in H4; simpl in H4;
+        clear H2 H3; destruct H4; destruct H2.
+        destruct H3 as [v_x H3]; exists v_x;
+        repeat split; destruct H3; destruct H4;
+        try rewrite lem_tsubBV_self; try apply IHn with Empty;
+        simpl in H; apply Nat.succ_le_mono in H;
+        try rewrite depth_tsubBV;
+        try apply Nat.le_trans with (max (depth t1) (depth t2));
+        try apply Nat.le_max_r;
+        try rewrite lem_erase_tsubBV;
+        try apply lem_ftyp_islc with FEmpty (erase t2);
+        inversion H0; try apply H5;
+        pose proof (fresh_not_elem (union nms (free t2))); 
+        set (y := fresh (union (nms) (free t2))) in H12;        
+        try rewrite lem_tsubFV_unbindT with y v_x t2;
+        apply lem_den_hasftype in H4 as H13;
+        try apply lem_subst_wf_top with t1;
+        apply not_elem_union_elim in H12; destruct H12;
+        try apply H11; simpl; auto. 
+      + (* Star *) simpl; apply H4.
+    * (* TPoly *) destruct k; simpl; apply H4.
+Qed.
 
-{-@ lem_denotations_selfify' :: t:UserType -> k:Kind -> ProofOf(WFType Empty t k)
-        -> { e:Term | Set_emp (freeBV e) } -> ProofOf(HasFType FEmpty e (erase t))
-        -> v:Value -> ProofOf(EvalsTo (App (App (AppT (Prim Eql) t) v) e) (Bc True))
-        -> ProofOf(Denotes t v) -> ProofOf(Denotes (self t e k) v) @-}
-lem_denotations_selfify' :: Type -> Kind -> WFType -> Expr -> HasFType -> Expr
-                                -> EvalsTo -> Denotes -> Denotes
-lem_denotations_selfify' t@(TRefn b z p)    Base p_emp_t e p_e_t v ev_rhs_tt den_t_v 
-  = lem_denotations_selfify_trefn' b z (p ? lem_refn_is_pred t b z p) p_emp_t 
-                                   e p_e_t v ev_rhs_tt den_t_v
-lem_denotations_selfify' (TFunc z t_z t')   k    p_emp_t e p_e_t v ev_rhs_tt den_t_v = den_t_v
-lem_denotations_selfify' (TPoly a k_a t')   k    p_emp_t e p_e_t v ev_rhs_tt den_t_v = den_t_v
-lem_denotations_selfify' t                  Star p_emp_t e p_e_t v ev_rhs_tt den_t_v = den_t_v
+Lemma lem_denotations_selfify : forall (t:type) (k:kind) (v:expr),
+    WFtype Empty t k -> HasFtype FEmpty v (erase t) -> isValue v
+        -> Denotes t v -> Denotes (self t v k) v.
+Proof. intros t k v p_emp_t. 
+  apply lem_denotations_selfify' with (depth t) Empty; trivial. Qed.
 
+Lemma lem_denotes_ctsubst_self : 
+  forall (th:csub) (t:type) (x:vname) (v':expr) (k:kind),
+    Denotes (self (ctsubst th t) (csubst th (FV x)) k) v'
+       -> Denotes (ctsubst th (self t (FV x) k)) v'.
+Proof. intro th; induction t; intros x v' k'; destruct k'; simpl;
+    try rewrite lem_ctsubst_func; try rewrite lem_ctsubst_exis;
+    try rewrite lem_ctsubst_poly; simpl; trivial.
+    - (* TRefn Base *)
 
-{-@ lem_equals_evals :: b:Basic -> z:RVname -> p:Pred -> e:Expr -> v:Value 
-        -> ProofOf(EvalsTo e v) -> ProofOf(HasFType FEmpty v (FTBasic b))
-        -> ProofOf(EvalsTo (App (App (AppT (Prim Eql) (TRefn b z p)) v) e) 
-                           (Bc True)) @-}
-lem_equals_evals :: Basic -> RVname -> Expr -> Expr -> Expr -> EvalsTo -> HasFType -> EvalsTo 
-lem_equals_evals TBool z p e v ev_e_v p_v_b = case v of -- b in {Bool,Int} is implicit here
-  (Bc w)  -> AddStep (App (App (AppT (Prim Eql) (TRefn TBool z p)) v) e) (App (App (Prim Eqv) v) e) step_one
-                           (Bc True) ev_eqv_tt
-    where
-      st_eql_eqv = EPrimT Eql (TRefn TBool z p) -- equals b ~> Prim Eqv
-      step_app   = EApp1 (AppT (Prim Eql) (TRefn TBool z p)) (Prim Eqv) st_eql_eqv v
-      step_one   = EApp1 (App (AppT (Prim Eql) (TRefn TBool z p)) v) (App (Prim Eqv) v) step_app e
-      ev_eqv_tt  = lemma_eqv_semantics v w (Refl v) e w ev_e_v
-  _       -> impossible ("by lemma" ? lem_bool_values v p_v_b)
-lem_equals_evals TInt  z p e v ev_e_v p_v_b = case v of
-  (Ic n) -> AddStep (App (App (AppT (Prim Eql) (TRefn TInt z p)) v) e) (App (App (Prim Eq) v) e) step_one
-                    (Bc True) ev_eq_tt
-    where
-      st_eql_eqv = EPrimT Eql (TRefn TInt z p) -- equals b ~> Prim Eq
-      step_app   = EApp1 (AppT (Prim Eql) (TRefn TInt z p)) (Prim Eq) st_eql_eqv v
-      step_one   = EApp1 (App (AppT (Prim Eql) (TRefn TInt z p)) v) (App (Prim Eq) v) step_app e
-      ev_eq_tt   = lemma_eq_semantics v n (Refl v) e n ev_e_v
-  _      -> impossible ("by lemma" ? lem_int_values v p_v_b)
-lem_equals_evals b     z p e v ev_e_v p_v_b = impossible ("by lemma" ? lem_base_types_star b p_emp_b)
-    where
-      p_emp_b = lem_ftyping_wfft FEmpty v (FTBasic b) p_v_b WFFEmpty
-
-{-@ lem_strengthen_evals_tt :: p1:Pred -> p2:Pred
-        -> ProofOf(HasFType FEmpty p1 (FTBasic TBool)) 
-        -> ProofOf(EvalsTo p1 (Bc True)) -> ProofOf(EvalsTo p2 (Bc True))
-        -> ProofOf(EvalsTo (strengthen p1 p2) (Bc True)) @-}
-lem_strengthen_evals_tt :: Expr -> Expr -> HasFType -> EvalsTo -> EvalsTo -> EvalsTo
-lem_strengthen_evals_tt p1 p2 pf_p1v_bl ev_p1v_tt ev_p2v_tt 
-  = lemma_strengthen_semantics p1 True ev_p1v_tt  p2 True ev_p2v_tt pf_p1v_bl
-
-{-@ lem_strengthen_evals_subBV :: p1:Pred -> p2:Pred -> v:Value
-        -> ProofOf(HasFType FEmpty (subBV 0 v p1) (FTBasic TBool)) 
-        -> ProofOf(EvalsTo (subBV 0 v p1) (Bc True)) -> ProofOf(EvalsTo (subBV 0 v p2) (Bc True)) 
-        -> ProofOf(EvalsTo (subBV 0 v (strengthen p1 p2)) (Bc True)) @-}
-lem_strengthen_evals_subBV :: Expr -> Expr -> Expr -> HasFType -> EvalsTo -> EvalsTo -> EvalsTo
-lem_strengthen_evals_subBV p1 p2 v pf_p1v_bl ev_p1v_tt ev_p2v_tt 
-  = lemma_strengthen_semantics (subBV 0 v p1) True ev_p1v_tt (subBV 0 v p2) True ev_p2v_tt pf_p1v_bl
-                               ? lem_subBV_strengthen  0 v p1 p2 
-*)
+    (* maybe try with subFTV first in the Basic Props Denotes file?*)
